theories/L/L_undec.v
@@ -7,6 +7,8 @@ Require Import Undecidability.L.Enumerators.term_enum.
 Require Import Undecidability.TM.TM.
 Require Import Undecidability.TM.TM_undec.
 Require Import Undecidability.L.Reductions.TM_to_L.
+Require Import Undecidability.MinskyMachines.MMA2_undec.
+Require Undecidability.L.Reductions.MMA_HALTING_to_HaltLclosed.
 
 (** ** HaltL is undecidable *)
 
@@ -15,4 +17,11 @@ Lemma HaltL_undec :
 Proof.
   apply (undecidability_from_reducibility HaltMTM_undec).
   eapply HaltMTM_to_HaltL.
+Qed.
+
+Lemma HaltLclosed_undec :
+  undecidable (HaltLclosed).
+Proof.
+  apply (undecidability_from_reducibility MMA2_HALTING_undec).
+  eapply MMA_HALTING_to_HaltLclosed.reduction.
 Qed.
